\begin{frame}[t,plain]
\titlepage
\end{frame}

% a hack, since colons do not render in the math environments
\renewcommand{\colon}{\mbox{~:~}}

\newcommand{\ang}[1]{\left\langle #1 \right\rangle}
\newcommand{\ceil}[1]{\left\lceil #1 \right\rceil}
\newcommand{\floor}[1]{\left\lfloor #1 \right\rfloor}
\renewcommand{\diamond}{\lozenge}
\newcommand{\T}{\mathfrak{T}}
\newcommand{\A}{\mathfrak{A}}
\renewcommand{\t}{\mathfrak{t}}
\newcommand{\e}{\mathfrak{e}}
\renewcommand{\v}{\mathfrak{v}}
\newcommand{\n}{\mathfrak{n}}
\newcommand{\dbrack}[1]{\left\llbracket #1 \right\rrbracket}

\newcommand{\angkv}{\langle k, v \rangle}
\newcommand{\angkvp}{\langle k', v' \rangle}

\begin{frame}[fragile]{Motivation}
    \begin{minted}{typescript}
  makePace(user: UserContext): Observable<boolean> {
    return this.complianceRuleLinkService
      .officiallyGetAllNeedingAHeartbeat(user)
      .pipe(projectToFormer())
      .pipe(flatMap(vertexId => this.deviceGroupService.getById(user, vertexId)))
      .pipe(map(vertex => vertex.deviceIds))
      .pipe(flatMap(deviceIds => this.deviceService.filterLastPushedAnciently(user, deviceIds, this.heartbeat)))
      .pipe(map(devices => devices.map(device => device.deviceId)))
      .pipe(tap(deviceIds => this.deviceService.updateLastPushed(user, deviceIds)))
      .pipe(flatMap(deviceIds => this.deviceCommandService.pushDevices(user, deviceIds)));
  }
    \end{minted}
\end{frame}

\begin{frame}[fragile]
    \frametitle{Main Goal}
  
    Verify linear-time temporal type theory, LTTT.
\end{frame}

\begin{frame}{Overview}
\tableofcontents
\end{frame}

\section{Preliminaries}

\subsection{Intuitionistic Propositional Logic}

\begin{frame}{Intuitionistic Logic}
    Intuitionistic propositional logic, IPL, differs from the classical one, by rejecting the law of excluded middle (\textit{principium tertii exclusi}).
    
    As a result, the following rules are not valid:
    \[
    \infer[\mbox{RAA}]{\Gamma \vdash \alpha}{\Gamma, \neg\alpha \vdash \bot}
    ~~~~ ~~~~
    \infer[\mbox{DNE}]{\Gamma \vdash \alpha}{\Gamma \vdash \neg\neg\alpha}
    \]
\end{frame}

\begin{frame}{Language of IPL}
    The language of IPL is defined by the following grammar:
    \[
    \alpha, \beta ::= \bot \mid a \mid \alpha \rightarrow \beta \mid \alpha \vee \beta \mid \alpha \wedge \beta,
    \]
    where
    \begin{itemize}
        \item $a$ ranges over atomic formulae,
        \item $\bot$ is contradiction or falsity,
        \item $\rightarrow$ is implication, $\vee$ is disjunction, and $\wedge$ is conjunction,
        \item $\neg\alpha$ is defined as $\alpha \rightarrow \bot$,
        \item $\top$ is defined as $\neg\bot$.
    \end{itemize}
\end{frame}

\begin{frame}[allowframebreaks]{IPL Inference Rules}
    The inference rules for IPL consists of the following (using natural deduction system with sequent):
    \begin{itemize}
        \item Axiom. $\Gamma, \alpha \vdash \alpha$.
        \item Principle of explosion (\textit{ex falso quodlibet}).
        \[
        \infer[\mbox{EFQ}]{\Gamma \vdash \beta}{\Gamma \vdash \bot}
        \]
        \item Implication rules.
        \[
        \infer[\rightarrow\mbox{-I}]{\Gamma \vdash \alpha \rightarrow \beta}{\Gamma, \alpha \vdash \beta}
        ~~~~ ~~~~
        \infer[\rightarrow\mbox{-E}]{\Gamma_1, \Gamma_2 \vdash \beta}{\Gamma_1 \vdash \alpha & \Gamma_2 \vdash \alpha \rightarrow \beta}
        \]
        \item Disjunction rules.
        \[
        \infer[\vee\mbox{-I}]{\Gamma\vdash \alpha_1 \vee \alpha_2}{\Gamma \vdash \alpha_i}
        ~~~~ ~~~~
        \infer[\vee\mbox{-E}]{\Gamma_1, \Gamma_2 \vdash \beta}{
            \Gamma_1 \vdash \alpha_1 \vee \alpha_2
            &
            \Gamma_2, \alpha_1 \vdash \beta
            &
            \Gamma_2, \alpha_2 \vdash \beta
        }
        \]
        \item Conjunction rules.
        \[
        \infer[\wedge\mbox{-I}]{\Gamma_1, \Gamma_2 \vdash \alpha_1 \wedge \alpha_2}{
            \Gamma_1 \vdash \alpha_1
            &
            \Gamma_2 \vdash \alpha_2
        }
        ~~~~ ~~~~
        \infer[\wedge\mbox{-E}]{\Gamma \vdash \alpha_i}{
            \Gamma \vdash \alpha_1 \wedge \alpha_2
        }
        \]
    \end{itemize}
    
    \begin{example}
    Prove that $\Gamma \vdash \top$ for all $\Gamma$.
    \end{example}
\end{frame}

\subsection{Curry--Howard Correspondence}

\begin{frame}{Simply Typed Lambda Calculus}
    The language of simply typed lambda calculus, TLC($\rightarrow$), is defined by:
    \begin{align*}
    \T, \mathfrak{S} &::= T \mid \T \rightarrow \mathfrak{S}, \\
    \t &::= x \mid \lambda x. \t \mid \t_1 \t_2.
    \end{align*}
    
    Typing rules consist of:
    \begin{itemize}
        \item Axiom. $\Gamma, x : \T \vdash x : \T$.
        \item Implication rules.
        \[
        \infer[\rightarrow\mbox{-I}]{\Gamma \vdash \lambda x. \t : \T \rightarrow \mathfrak{S}}{\Gamma, x : \T \vdash \t : \mathfrak{S}}
        ~~~~ ~~~~
        \infer[\rightarrow\mbox{-E}]{\Gamma \vdash \t_1\t_2 : \mathfrak{S}}{
            \Gamma \vdash \t_1 : \T \rightarrow \mathfrak{S}
            &
            \Gamma \vdash \t_2 : \T
        }
        \]
    \end{itemize}
\end{frame}

\begin{frame}{More Types}
\begin{itemize}
    \item Unit type, is a type inhabited by a single term.
    \begin{tabular}{l|cc}
        Language & Type & Value \\
        \hline
        Scala & \texttt{Unit} & \texttt{()} \\
        Haskel, Rust, Swift & \texttt{()} & \texttt{()} \\
        ML, OCaml, F\# & \texttt{unit} & \texttt{()} \\
        TypeScript & \texttt{undefined} & \texttt{undefined}
    \end{tabular}
    \item A bottom type, is a type that has no value. E.g. \texttt{Nothing} in Scala and \texttt{never} or \texttt{void} in TypeScript.
    \item Union type (aka tagged union or sum type) is a union of other types. The actual type is usually decided in the runtime by pattern matching.
    
    \texttt{type Tree = Node | Leaf;}
    \item Product type is usually realized as the type of tuples.
    
\end{itemize}
\end{frame}

\begin{frame}[allowframebreaks]{Extending Simply Typed Lambda Calculus}
    One can extend TLC($\rightarrow$) by adding tuples, unions, and unit and bottom type:
    \begin{align*}
    i ::=&~ 1 \mid 2, \\
    \T, \mathfrak{S} ::=&~ T \mid \mathtt{Unit} \mid \mathtt{Void} \mid \T \rightarrow \mathfrak{S} \mid \T \times \mathfrak{S} \mid \T + \mathfrak{S}, \\
    \t ::=&~ x \mid \lambda x. \t \mid \t_1 \t_2 \mid () \mid (\t_1, \t_2) \mid \pi_i(\t) \mid \iota_i(\t) \\ &\mid \mathtt{case}~\t~\mathtt{of}~(\iota_1 x_1 \rightarrow \t_1 \mid \iota_2 x_2 \rightarrow \t_2) \\
    &\mid \mathtt{case}~\t~\mathtt{of}~().
    \end{align*}
    
    The additional rules are:
    \begin{itemize}
        \item Unit and bottom type rules.
        \[
        \infer[\mathtt{Unit}\mbox{-I}]{\Gamma \vdash () : \mathtt{Unit}}{}
        ~~~~ ~~~~
        \infer[\mathtt{Void}\mbox{-E}]{\Gamma \vdash \mathtt{case}~\t~\mathtt{of}~() : \mathfrak{S}}{\Gamma \vdash \t : \mathtt{Void}}
        \]
        \item Tuple rules.
        \[
        \infer[\times\mbox{-I}]{\Gamma \vdash (\t_1, \t_2) : \T_1 \times \T_2}{\Gamma \vdash \t_1 : \T_1 & \Gamma \vdash \t_2 : \T_2}
        ~~~~ ~~~~
        \infer[\times\mbox{-E}]{\Gamma \vdash \pi_i \t : \T_i}{\Gamma \vdash \t : \T_1 \times \T_2}
        \]
        \item Union type rules.
        \begin{gather*}
        \infer[+\mbox{-I}]{\Gamma \vdash \iota_i \t : \T_1 + \T_2}{\Gamma \vdash \t : \T_i}
        \\ \\
        \infer[+\mbox{-E}]{\Gamma \vdash \mathtt{case}~\t~\mathtt{of}~(\iota_1 x_1 \rightarrow \t_1 \mid \iota_2 x_2 \rightarrow \t_2) : \mathfrak{S}}{
            \Gamma \vdash \t : \T_1 + \T_2
            &
            \Gamma, x_1 : \T_1 \vdash \t_1 : \mathfrak{S}
            &
            \Gamma, x_2 : \T_2 \vdash \t_2 : \mathfrak{S}
        }
        \end{gather*}
    \end{itemize}
    
    We call the extended TLC($\rightarrow$), TLC($\rightarrow, \times, +, \mathtt{Unit}, \mathtt{Void}$) or simply TLC.
\end{frame}

\begin{frame}{Curry--Howard Correspondence}
\begin{theorem}[\cite{Howard1969TheFN}]
The types in $\mathrm{TLC}$ form an $\mathrm{IPL}$. Furthermore:
\begin{itemize}
    \item If $\Gamma \vdash \t : \alpha$ then $\pi_2[\Gamma] \vdash \alpha$,
    \item If $\Delta \vdash \alpha$ then there is a $\Gamma$ and a $\t$ that $\Delta = \pi_2[\Gamma]$ and $\Gamma \vdash \t : \alpha$.
\end{itemize}
\end{theorem}
\end{frame}

\subsection{Linear Logic}

\begin{frame}{Structural Rules}
    \begin{itemize}
        \item \textbf{Weakening}. Which states that hypotheses of a sequent could be extended.
        \begin{gather*}
            \infer=[\mbox{Weak}]{\Gamma_1, \alpha, \Gamma_2 \vdash \beta}{\Gamma_1, \Gamma_2 \vdash \beta}
            ~~~~ ~~~~
            \infer=[\mbox{Weak}]{\Gamma_1, x : \A, \Gamma_2\vdash \t : \mathfrak{B}}{\Gamma_1, \Gamma_2\vdash \t : \mathfrak{B}}
        \end{gather*}
        \item \textbf{Contraction}. Which states that two similar (or unifiable) hypotheses can be replaced by a single hypothesis.
        \begin{gather*}
            \infer=[\mbox{Contr}]{\Gamma_1, \alpha, \Gamma_2 \vdash \beta}{\Gamma_1, \alpha, \alpha, \Gamma_2 \vdash \beta}
            ~~~~ ~~~~
            \infer=[\mbox{Contr}]{\Gamma_1, x : \A, \Gamma_2 \vdash \t : \mathfrak{B}}{\Gamma_1, x : \A, x : \A, \Gamma_2 \vdash \t : \mathfrak{B}}
        \end{gather*}
        \item \textbf{Exchange}. Which states that two hypotheses may be swapped.
        \begin{gather*}
            \infer=[\mbox{Exch}]{\Gamma_1, \alpha_2, \alpha_1, \Gamma_2 \vdash \beta}{\Gamma_1, \alpha_1, \alpha_2, \Gamma_2 \vdash \beta}
            ~~~~ ~~~~
            \infer=[\mbox{Exch}]{\Gamma_1, x_2 : \A_2, x_1 : \A_1 \Gamma_2 \vdash \t : \mathfrak{B}}{\Gamma_1, x_1 : \A_1, x_2 : \A_2, \Gamma_2 \vdash \t : \mathfrak{B}}
        \end{gather*}
    \end{itemize}
\end{frame}

\begin{frame}{Substructural Logics / Type Systems}
    \begin{table}[!ht]
    \centering
    \begin{tabular}{l|ccc}
         & W & C & E \\
        \hline
        Unrestricted & \checkmark & \checkmark & \checkmark \\
        Affine & \checkmark &  & \checkmark \\
        Relevant &  & \checkmark & \checkmark \\
        Linear & & & \checkmark \\
        Ordered
    \end{tabular}
    \caption{Substructural logics / type systems}
    \label{tab:my_label}
\end{table}

\begin{itemize}
    \item \textbf{Affine}. Every variable can be used at most once.
    \item \textbf{Relevant}. Every variable must be used at least once.
    \item \textbf{Linear}. Every variable must be used exactly once.
    \item \textbf{Ordered}. Every variable must be used exactly once and in the order in which it is introduced.
\end{itemize}
\end{frame}

\begin{frame}{Linear Logic}
    The linear logic \cite{DBLP:journals/tcs/Girard87}, LL$(0, \multimap, \oplus, \otimes, !)$ or simply LL, consists of the following language:
    \[
    \alpha ::= 0 \mid a \mid \alpha \multimap \alpha \mid \alpha \oplus \alpha \mid \alpha \otimes \alpha \mid~ !\alpha.
    \]
    
    \begin{itemize}
        \item $0$ is linear version of $\bot$,
        \item $!$ is called \textit{of course} or \textit{bang} and makes the formulae non-linear,
        \item $\multimap$ is bilinear version of implication,
        \item $\oplus$ is called \textit{additive disjunction} is the bilinear version of or,
        \item $\otimes$ is called \textit{multiplicative conjunction} or \textit{tensor} is the bilinear version of and.
    \end{itemize}
\end{frame}

\begin{frame}{Linear/Non-Linear Logic}
    The linear/non-linear logic \cite{DBLP:conf/csl/Benton94}, or simply LNL, consists of the following language:
    \begin{align*}
        &\tau ::= \bot \mid t \mid \tau \times \tau \mid \tau + \tau \mid \tau \rightarrow \tau \mid \ceil{\alpha}, \\
        &\alpha ::= 0 \mid a \mid \alpha \otimes \alpha \mid \alpha \oplus \alpha \mid \alpha \multimap \alpha \mid \floor{\tau}.
    \end{align*}
    \begin{itemize}
        \item $\ceil{\cdot}$ is called \textit{lift},
        \item $\floor{\cdot}$ is called \textit{lower}.
    \end{itemize}
\end{frame}

\subsection{Temporal Logic}

\begin{frame}{Modal Logic}
    The language of the modal logic is defined by the following grammar:
    \[
    \alpha ::= \bot \mid a \mid \alpha \rightarrow \alpha \mid \alpha \vee \alpha \mid \alpha \wedge \alpha \mid \diamond\alpha \mid \square\alpha.
    \]
    
    \begin{itemize}
        \item $\diamond\varphi$ reads ``possibly $\varphi$'',
        \item $\square\varphi$ reads ``necessarily $\varphi$''.
    \end{itemize}
\end{frame}

\begin{frame}{Temporal Logic}
    Formulating temporal logic as a modal logic was first done by Prior \cite{PRIOR1957,PRIOR1967,prior1968papers} and then ported to computer science by Pnueli \cite{DBLP:conf/focs/Pnueli77}.
    
    \begin{itemize}
        \item $\diamond\varphi$ reads ``it will at some time be the case that $\varphi$''.
        \item $\square\varphi$ reads ``it will always be the case that $\varphi$''.
    \end{itemize}
\end{frame}

\begin{frame}{Linear-Time Temporal Logic}
    Linear-time temporal logic \cite{DBLP:conf/focs/Pnueli77}, or LTL, reasons about linear time.
    
    Some properties of LTL:
    \begin{itemize}
        \item Future and always are dual:
        \begin{eqnarray*}
        \neg\diamond\varphi &\equiv& \square\neg\varphi, \\
        \neg\square\varphi &\equiv& \diamond\neg\varphi.
        \end{eqnarray*}
        \item $\square\varphi \rightarrow \square\square\varphi$,
        \item $\square\square\varphi \rightarrow \square\varphi$,
        \item $\diamond\varphi \rightarrow \diamond\diamond\varphi$, 
        \item $\diamond\diamond\varphi \rightarrow \diamond\varphi$.
    \end{itemize}
\end{frame}

\section{Linear-Time Temporal Type Theory}

\begin{frame}[allowframebreaks]{Linear-Time Temporal Type Theory}
    The linear-time temporal type theory \cite{Paykin2016TheEO} consists of the following language:

    \begin{align*}
        \T ::=&~ \mathtt{Unit} \mid \mathtt{Void} \mid \T \times \T \mid \T + \T \mid \T \rightarrow \T \mid \ceil{\A} \\
        \A ::=&~ 1 \mid 0 \mid \A \otimes \A \mid \A \oplus \A \mid \A \multimap \A \mid \diamond\A \mid \floor{\T} \\
        \\
        \t ::=&~ x \mid () \mid \mathtt{case}~\t~\mathtt{of}~() \mid (\t_1, \t_2) \mid \pi_i \t \mid \iota_i \t \mid \mathtt{case}~\t~\mathtt{of}~(\iota_1 x_1 \rightarrow \t_1 \mid \iota_2 x_2 \rightarrow \t_2) \\
        & \mid \lambda x. \t \mid \t_1 \t_2 \mid \mathtt{suspend}~\e \\
        \e ::=&~ x \mid () \mid \mathtt{case}~\e~\mathtt{of}~() \mid (\e_1, \e_2) \mid \iota_i \e \mid \mathtt{case}~\t~\mathtt{of}~(\iota_1 x_1 \rightarrow \e_1 \mid \iota_2 x_2 \rightarrow \e_2) \\
        & \mid \lambda x. \e \mid \e_1 \e_2 \mid \mathtt{force}~\t \mid \mathtt{return}~\e \mid \mathtt{bind}~x = \e_1~\mathtt{in}~\e_2 \mid \floor{\t} \\
        &\mid \mathtt{let}~() = \e_1~\mathtt{in}~\e_2 \mid \mathtt{let}~(x_1, x_2) = \e_1~\mathtt{in}~\e_2 \mid \mathtt{let}~\floor{x} = \e_1~\mathtt{in}~\e_2
    \end{align*}

    \begin{itemize}
        \item Lift and lower rules.
        \begin{gather*}
        \infer[\ceil{\cdot}\mbox{-I}]{\Gamma \vdash \mathtt{suspend}~\e : \ceil{\A}}{\Gamma; \cdot \vdash \e : \A}
        ~~~~ ~~~~
        \infer[\ceil{\cdot}\mbox{-E}]{\Gamma; \cdot \vdash \mathtt{force}~\t : \A}{\Gamma \vdash \t : \ceil{\A}}
        \\ \\ 
        \infer[\floor{\cdot}\mbox{-I}]{\Gamma; \cdot \vdash \floor{\t} : \floor{\T}}{\Gamma \vdash \t : \T}
        ~~~~ ~~~~
        \infer[\floor{\cdot}\mbox{-E}]{\Gamma; \Delta_1, \Delta_2 \vdash \mathtt{let}~\floor{x} = \e_1~\mathtt{in}~\e_2 : \mathfrak{B}}{
            \Gamma; \Delta_1 \vdash \e_1 : \floor{\T}
            &
            \Gamma, x : \T; \Delta_2 \vdash \e_2 : \mathfrak{B}
        }
        \end{gather*}
    \end{itemize}
\end{frame}

\begin{frame}[allowframebreaks]{LTTT Operational Semantics}
    The operational semantics using context hole consists of normal versions of $\t$ and $\e$, a relation $\leadsto$, evaluation contexts $\mathfrak{E}_\t$ and $\mathfrak{E}_\e$, and reduction rules.
    
    \begin{itemize}
        \item Normal terms and expressions.
        \begin{align*}
            \v ::=&~ () \mid (\v_1, \v_2) \mid \iota_i \v \mid \lambda x. \t \mid \mathtt{suspend}~\e \\
            \n ::=&~ () \mid (\e_1, \e_2) \mid \iota_i \e \mid \lambda x. \e \mid \mathtt{return}~\e \mid \floor{\v}
        \end{align*}
    
        \item The step relation.
        \begin{eqnarray*}
        \pi_i(\v_1, \v_2) &\leadsto& \v_i\\
        (\lambda x.\t_1)\v_2 &\leadsto& \t_1 [x \mapsto \v_2]\\
        \mathtt{case}\ \ \iota_i\v \ \ \mathtt{of}\ (\iota_1\ x_1 \mapsto \t_1\  \lvert\  \iota_2 \ x_2 \ \mapsto \t_2) &\leadsto& \t_i [x_i \mapsto \v]\\
        \mathtt{let}\ ()=()\ \mathtt{in} \ \e &\leadsto& \e\\
        \mathtt{let}\ (x_1,x_2)=(\e_1,\e_2)\ \mathtt{in}\ \e &\leadsto& \e[x_1 \mapsto \e_1, x_2 \mapsto \e_2]\\
        (\lambda x.\e_1)\e_2 &\leadsto& \e_1[x \mapsto \e_2]\\
        \mathtt{bind}\ x = \mathtt{return} \ \e_1\ \mathtt{in} \ \e_2\ &\leadsto&\ \e_2 [x \mapsto \e_1]\\
        \mathtt{force}( \mathtt{suspend}\ \e)\ &\leadsto& \e\\
        \mathtt{let}\  \floor{x}=\floor{\v}\  \mathtt{in}\ \e\ &\leadsto& \e[x\mapsto \v]\\
        \mathtt{case}\ \ \iota_i\e \ \ \mathtt{of}\ (\iota_1\ x_1 \mapsto \e_1\  \lvert\  \iota_2 \ x_2 \mapsto \e_2) &\leadsto& \e_i [x_i \mapsto \e]
        \end{eqnarray*}
        
        \item Evaluation context.
        \begin{align*}
            \mathfrak{E}_{\t} ::=&~ ([~], \t) \mid (\v, [~]) \mid \pi_i [~] \mid \iota_i [~] \\
            & \mid \mathtt{case}~[~]~\mathtt{of}~(\iota_1 x_1 \rightarrow \t_1 \mid \iota_2 x_2 \rightarrow \t_2) \\
            & \mid [~] \t \mid \v [~] \mid \mathtt{force}~[~] \mid \floor{[~]} \\
            \mathfrak{E}_\e ::=&~ \mathtt{let}~() = [~]~\mathtt{in}~\e \mid \mathtt{let}~(x_1, x_2) = [~]~\mathtt{in}~\e \\
            & \mid \mathtt{case}~[~]~\mathtt{of}~(\iota_1 x_1 \rightarrow \e_1 \mid \iota_2 x_2 \rightarrow \e_2) \\
            & \mid [~] \e \mid \mathtt{bind}~x = [~]~\mathtt{in}~\e \mid \mathtt{let}~\floor{x} = [~]~\mathtt{in}~\e
        \end{align*}
        
        \item Reduction rules.
        \[
        \infer{\mathfrak{E}_\t \dbrack{\t} \leadsto \mathfrak{E}_\t \dbrack{\t'}}{\t \leadsto \t'}
        ~~~~ ~~~~
        \infer{\mathfrak{E}_\e \dbrack{\e} \leadsto \mathfrak{E}_\e \dbrack{\e'}}{\e \leadsto \e'}
        \]
    \end{itemize}
\end{frame}

\section{Coq Implementation}

\begin{frame}{Coq Implementation}
    The Coq implementation consists of:
    \begin{itemize}
        \item A generic store, used as the typing context,
        \item LTTT typing rules and operational semantics.
    \end{itemize}
    
    Two more typing rules are introduced for typing substitution:
    \[
    \infer[\mbox{$\t$-Subst}]{\Gamma \vdash \t[x \mapsto \t'] : \T}{
    \Gamma, x : \T' \vdash \t : \T
    &
    \Gamma \vdash \t' : \T'
    }
    \]
    \[
    \infer[\mbox{$\e$-Subst}]{\Gamma; \Delta_1, \Delta_2 \vdash \e[x \mapsto \e'] : \A}{
    \Gamma; \Delta_1, x : \A' \vdash \e : \A
    &
    \Gamma; \Delta_2 \vdash \e' : \A'
    }
    \]
\end{frame}

\begin{frame}{Coq Implementation Results}
    Two results are proved in Coq:
    
    \begin{lemma}[$\t$-Preservation]
    \label{lemma:t-preservation}
    For all $\Gamma, \t, \t', \T$, if $\Gamma \vdash \t : \T$ and $\t \leadsto \t'$, then $\Gamma \vdash \t' : \T$.
    \end{lemma}
    
    \begin{lemma}[Weak $\e$-Preservation]
    \label{lemma:e-preservation-weak}
    For all $\e, \e', \A$, if $\vdash \e : \A$ and $\e \leadsto \e'$, then $\vdash \e' : \A$.
    \end{lemma}
\end{frame}

\subsection{Generic Store}

\begin{frame}[allowframebreaks]{Generic Store}
    Generic store is a the data structure used for the typing context.
    \[
    S ::= \emptyset~|~S :: \angkv.
    \]
    
    \begin{itemize}
        \item Concatenation.
        \[
        S \circ S' =
        \begin{cases}
            S, & S' = \emptyset, \\
            (S \circ S'') :: \angkv, & S' = S'' :: \angkv.
        \end{cases}
        \]
        
        \item Membership.
        \begin{itemize}
            \item If $S = S' :: \angkv$, then $\angkv \in S$,
            \item If $\angkvp \in S'$ and $k \not= k'$, then $\angkvp \in S :: \angkv$. \qedhere
        \end{itemize}
    \end{itemize}
    
    \begin{lemma}
    Let $B$ and $C$ be stores, $k$ a key, and $v$ a value. Then:
    \begin{itemize}
        \item If $\angkv \in C$, then $\angkv \in B \circ C$,
        \item If $\angkv \in B$ and $\ang{k, \cdot} \not\in C$, then $\angkv \in B \circ C$,
        \item If $\angkv \in B \circ C$, then either $\angkv \in B$ or $\angkv \in C$.
    \end{itemize}
    \end{lemma}
    
    \begin{definition}[Equivalence]
        \begin{itemize}
            \item If for every $\angkv \in S$ we have $\angkv \in S'$, we write $S \sqsubseteq S'$.
            \item If $S \sqsubseteq S'$ and $S' \sqsubseteq S$, we write $S \equiv S'$ and say they are equivalent.
        \end{itemize}
    \end{definition}
    
    \begin{axiom}[Extensionality]
        If $B \equiv C$ then $B = C$.
    \end{axiom}
    
    \begin{theorem}[Exchange]
    For stores $A, B, C, D$, if $B \circ C$ is has no duplicate keys, then $A \circ B \circ C \circ D = A \circ C \circ B \circ D$.
    \end{theorem}
    
    \begin{corollary}[Append Commute]
    For any store $S$, keys $k, k'$, and values $v, v'$, if $k \not= k'$, then $S :: \ang{k, v} :: \ang{k', v'} = S :: \ang{k', v'} :: \ang{k, v}$.
    \end{corollary}
    \begin{proof}
    By writing $S :: \ang{k, v} :: \ang{k', v'}$ as $S \circ (\emptyset :: \ang{k, v}) \circ (\emptyset :: \ang{k', v'})$, realizing that $(\emptyset :: \ang{k, v}) \circ (\emptyset :: \ang{k', v'})$ is unique-paired, and then using exchange.
    \end{proof}
\end{frame}

\begin{frame}[fragile]{Coq Proof of Append Commute}
    \begin{minted}[fontsize=\small]{coq}
Proposition append_commut : forall s k v k' v',
  unique_paired (append empty k v o append empty k' v') ->
  append (append s k v) k' v' = append (append s k' v') k v.
Proof.
  intros. rewrite -> append_to_concat.
  rewrite -> append_to_concat.
  rewrite <- id_r with
    (m := s o (append empty k v) o (append empty k' v')).
  rewrite -> exchange; auto. rewrite -> id_r.
  repeat rewrite <- append_to_concat.
  reflexivity.
Qed.
    \end{minted}
\end{frame}

\section{TypeScript Implementation}

\begin{frame}[t,allowframebreaks]
\nocite{*}
\frametitle{References}
\bibliographystyle{apalike}
\bibliography{ref.bib}
\end{frame}
